*** empty log message ***

examples/dev/sw/preARMScript.sml
@@ -4,27 +4,6 @@ open HolKernel Parse boolLib bossLib numLib pred_setSimps pred_setTheory
 val _ = new_theory "preARM";
 
 (*----------------------------------------------------------------------------*)
-(* Preprocessing                                                              *)
-(*----------------------------------------------------------------------------*)
-
-(*
-val _ = add_rule{term_name   = "COND",
-fixity      = Infix (HOLgrammars.RIGHT, 3),
-pp_elements = [HardSpace 1, TOK "=>", BreakSpace(1,0), TM, BreakSpace(1,0), TOK "|", HardSpace 1],
-paren_style = OnlyIfNecessary,
-block_style = (AroundEachPhrase, (PP.INCONSISTENT, 0))};
-*)
-
-(*
-val _ = add_rule{term_name   = "COND",
-fixity      = TruePrefix 70,
-pp_elements = [PPBlock([TOK "if", BreakSpace(1,2), TM, BreakSpace(1,0),TOK "then"], (CONSISTENT, 0)),
-	       BreakSpace(1,2), TM, BreakSpace(1,0), TOK "else", BreakSpace(1,2)],
-paren_style = Always,
-block_style = (AroundEachPhrase, (PP.CONSISTENT, 0))};
-*)
-
-(*----------------------------------------------------------------------------*)
 (* Registers	                                                              *)
 (*----------------------------------------------------------------------------*)
 
@@ -89,8 +68,7 @@ val _ = Hol_datatype ` OPERATOR = MOV |
                         LSL | LSR | ASR | ROR |
                         LDR | STR | LDMFD | STMFD |
                         MRS | MSR |
-                        B | BL |
-                        SWI
+                        B | BL
              `;
 
 (*-------------------------------------------------------------------------------*)
@@ -104,6 +82,7 @@ val _ = Hol_datatype ` COND = EQ | NE | GE | LE | GT | LT | AL | NV`;
 (*-------------------------------------------------------------------------------*)
 
 val _ = type_abbrev("ADDR", Type`:num`);
+val _ = type_abbrev("DATA", Type`:word32`);
 
 val _ = Hol_datatype `OFFSET = POS of ADDR
                | NEG of ADDR
@@ -116,10 +95,22 @@ val _ = Hol_datatype `EXP = MEM of num # OFFSET			(* (register, offset) *)
 		  | WCONST of word32
                   | REG of REGISTER
 		  | WREG of REGISTER
-                  | PR of EXP # EXP
              `;
 
-val _ = type_abbrev("DATA", Type`:word32`);
+val FP_def =
+  Define `FP = REG 11`;
+
+val IP_def =
+  Define `IP = REG 12`;
+
+val SP_def =
+  Define `SP = REG 13`;
+
+val LR_def =
+  Define `LR = REG 14`;
+
+val PC_def =
+  Define `PC = REG 15`;
 
 (*-------------------------------------------------------------------------------*)
 (* Operations                                                                    *)
@@ -135,10 +126,10 @@ val _ = type_abbrev("INST", Type`:OPERATION # (EXP option) # (EXP list) # (OFFSE
   
 val _ = type_abbrev("STATE", Type`: ADDR # CPSR # (REGISTER |-> DATA) # (ADDR |-> DATA)`);
 
-val FORALL_STATUS = Q.store_thm
-  ("FORALL_STATUS",
-    `(!s:CPSR # (REGISTER |-> DATA) # (ADDR |-> DATA). P s) = 
-	!pcsr regs mem. P (pcsr,(regs,mem))`,
+val FORALL_DSTATE = Q.store_thm
+  ("FORALL_DSTATE",
+    `(!s:(REGISTER |-> DATA) # (ADDR |-> DATA). P s) = 
+	!regs mem. P (regs,mem)`,
     SIMP_TAC std_ss [FORALL_PROD]);
 
 val FORALL_STATE = Q.store_thm
@@ -170,19 +161,9 @@ val read_thm = Q.store_thm (
     (read (regs,mem) (MEM (r,NEG k)) = mem ' (w2n (regs ' r) - k)) /\
     (read (regs,mem) (NCONST i) = n2w i) /\
     (read (regs,mem) (WCONST w) = w) /\
-    (read (regs,mem) (REG r) = regs ' r)`,
+    (read (regs,mem) (REG r) = regs ' r) /\
+    (read (regs,mem) (MEM (r,INR)) = ARB)`,
     RW_TAC std_ss [read_def]);
-
-
-val mread_def =
-  Define `
-    ( mread s (PR (exp1,exp2)) = 
-         PR (mread s exp1, mread s exp2)
-    ) /\
-    ( mread s exp = 
-         WCONST (read s exp)
-    )
-  `;
 
 val write_def =
   Define `
@@ -203,31 +184,9 @@ val write_thm = Q.store_thm (
   "write_thm",
   ` (write (regs,mem) (MEM (r,POS k)) v = (regs, mem |+ (w2n (regs ' r) + k, v))) /\
     (write (regs,mem) (MEM (r,NEG k)) v = (regs, mem |+ (w2n (regs ' r) - k, v))) /\
+    (write (regs,mem) (MEM (r,INR)) v = (regs,ARB)) /\
     (write (regs,mem) (REG r) v = (regs |+ (r, v), mem))`,
     RW_TAC std_ss [write_def]);                      
-
-
-val mwrite_def =
-  Define `
-    ( mwrite s (PR (pos1,pos2)) (PR (v1,v2)) = 
-         mwrite (mwrite s pos1 v1) pos2 v2) /\
-    ( mwrite s exp (WCONST v) = 
-         write s exp v)
-  `;
-
-
-val mwrite_thm = Q.prove (
-  ` ( mwrite s (PR (pos1,pos2)) (PR (v1,v2)) = 
-         mwrite (mwrite s pos1 v1) pos2 v2) /\
-    ( mwrite s (REG r) (WCONST v) = 
-         write s (REG r) v) /\
-    ( mwrite s (WREG r) (WCONST v) = 
-         write s (WREG r) v) /\
-    ( mwrite s (MEM m) (WCONST v) = 
-         write s (MEM m) v)`,
-  RW_TAC std_ss [mwrite_def]
- );
-
 
 (*---------------------------------------------------------------------------------*)
 (* Decoding and execution of an instruction                                        *)
@@ -251,20 +210,9 @@ val goto_thm = Q.store_thm (
   RW_TAC std_ss [goto_def]);
 
 
-val read_pc = 
+val decode_op_def = 
   Define `
-    read_pc (cpsr,s) = 
-		(w2n (read s (REG 15)), cpsr, s)`;
-
-val set_pc =
-  Define `
-    set_pc s pc =
-                (pc, FST s, write (SND s) (REG 15) (n2w pc))`;
-
-
-val decode1_def = 
-  Define `
-  decode1 (pc,cpsr,s) (op,dst,src,jump) =
+  decode_op (pc,cpsr,s) (op,dst,src,jump) =
      case op of
           MOV -> (cpsr, write s (THE dst) (read s (HD src)))
               ||
@@ -346,45 +294,42 @@ val decode1_def =
           MRS -> (cpsr, (write s (THE dst) cpsr))
 	      ||
 
-	  B   -> (cpsr, write s (REG 15) (n2w (goto(pc,jump))))
+	  B   -> (cpsr, s)
 	      || 
-          BL ->  (cpsr, write (write s (REG 14) (n2w (pc+1))) (REG 15) (n2w (goto(pc,jump))))
-              ||
-
-          _  ->  ARB
+          BL ->  (cpsr, write s (REG 14) (n2w (SUC pc)))
   `;
 
-val decode1_thm = Q.store_thm
-("decode1_thm",
+val decode_op_thm = Q.store_thm
+("decode_op_thm",
   `!pc cpsr s dst src jump.
-  (decode1 (pc,cpsr,s) (MOV,SOME dst,src,jump) = (cpsr, write s dst (read s (HD src)))) /\
-  (decode1 (pc,cpsr,s) (ADD,SOME dst,src,jump) = (cpsr, write s dst (read s (HD src) + read s (HD (TL src))))) /\
-  (decode1 (pc,cpsr,s) (SUB,SOME dst,src,jump) = (cpsr, write s dst (read s (HD src) - read s (HD (TL src))))) /\
-  (decode1 (pc,cpsr,s) (RSB,SOME dst,src,jump) = (cpsr, write s dst (read s (HD (TL src)) - read s (HD src)))) /\
-  (decode1 (pc,cpsr,s) (MUL,SOME dst,src,jump) = (cpsr, write s dst (read s (HD src) * read s (HD (TL src))))) /\
-  (decode1 (pc,cpsr,s) (MLA,SOME dst,src,jump) = (cpsr, write s dst (read s (HD src) * read s (HD (TL src)) + read s (HD (TL (TL src)))))) /\
-  (decode1 (pc,cpsr,s) (AND,SOME dst,src,jump) = (cpsr, write s dst (read s (HD src) & read s (HD (TL src))))) /\
-  (decode1 (pc,cpsr,s) (ORR,SOME dst,src,jump) = (cpsr, write s dst (read s (HD src) | read s (HD (TL src))))) /\
-  (decode1 (pc,cpsr,s) (EOR,SOME dst,src,jump) = (cpsr, write s dst (read s (HD src) # read s (HD (TL src))))) /\
-  (decode1 (pc,cpsr,s) (CMP,NONE,src,jump) = (if read s (HD src) = read s (HD (TL src))
+  (decode_op (pc,cpsr,s) (MOV,SOME dst,src,jump) = (cpsr, write s dst (read s (HD src)))) /\
+  (decode_op (pc,cpsr,s) (ADD,SOME dst,src,jump) = (cpsr, write s dst (read s (HD src) + read s (HD (TL src))))) /\
+  (decode_op (pc,cpsr,s) (SUB,SOME dst,src,jump) = (cpsr, write s dst (read s (HD src) - read s (HD (TL src))))) /\
+  (decode_op (pc,cpsr,s) (RSB,SOME dst,src,jump) = (cpsr, write s dst (read s (HD (TL src)) - read s (HD src)))) /\
+  (decode_op (pc,cpsr,s) (MUL,SOME dst,src,jump) = (cpsr, write s dst (read s (HD src) * read s (HD (TL src))))) /\
+  (decode_op (pc,cpsr,s) (MLA,SOME dst,src,jump) = (cpsr, write s dst (read s (HD src) * read s (HD (TL src)) + read s (HD (TL (TL src)))))) /\
+  (decode_op (pc,cpsr,s) (AND,SOME dst,src,jump) = (cpsr, write s dst (read s (HD src) & read s (HD (TL src))))) /\
+  (decode_op (pc,cpsr,s) (ORR,SOME dst,src,jump) = (cpsr, write s dst (read s (HD src) | read s (HD (TL src))))) /\
+  (decode_op (pc,cpsr,s) (EOR,SOME dst,src,jump) = (cpsr, write s dst (read s (HD src) # read s (HD (TL src))))) /\
+  (decode_op (pc,cpsr,s) (CMP,NONE,src,jump) = (if read s (HD src) = read s (HD (TL src))
                                              then (setS 0w SZ,s)
                                              else (if read s (HD src) <. read s (HD (TL src))
                                                    then (setS 0w SN,s)
                                                    else (setS 0w SC,s)))) /\
-  (decode1 (pc,cpsr,s) (TST,NONE,src,jump) = (if read s (HD src) & read s (HD (TL src)) = 0w
+  (decode_op (pc,cpsr,s) (TST,NONE,src,jump) = (if read s (HD src) & read s (HD (TL src)) = 0w
                                              then (setS cpsr SZ,s) else (cpsr,s))) /\
-  (decode1 (pc,cpsr,s) (LSL,SOME dst,src,jump) = (cpsr, write s dst (read s (HD src) << w2n (read s (HD (TL src)))))) /\
-  (decode1 (pc,cpsr,s) (LSR,SOME dst,src,jump) = (cpsr, write s dst (read s (HD src) >>> w2n (read s (HD (TL src)))))) /\
-  (decode1 (pc,cpsr,s) (ASR,SOME dst,src,jump) = (cpsr, write s dst (read s (HD src) >> w2n (read s (HD (TL src)))))) /\
-  (decode1 (pc,cpsr,s) (ROR,SOME dst,src,jump) = (cpsr, write s dst (read s (HD src) #>> w2n (read s (HD (TL src)))))) /\
-  (decode1 (pc,cpsr,s) (LDR,SOME dst,src,jump) = (cpsr, write s dst (read s (HD src)))) /\
-  (decode1 (pc,cpsr,s) (STR,SOME dst,src,jump) = (cpsr, write s (HD src) (read s dst))) /\
-  (decode1 (pc,cpsr,s) (LDMFD, SOME (REG r),src,jump) =
+  (decode_op (pc,cpsr,s) (LSL,SOME dst,src,jump) = (cpsr, write s dst (read s (HD src) << w2n (read s (HD (TL src)))))) /\
+  (decode_op (pc,cpsr,s) (LSR,SOME dst,src,jump) = (cpsr, write s dst (read s (HD src) >>> w2n (read s (HD (TL src)))))) /\
+  (decode_op (pc,cpsr,s) (ASR,SOME dst,src,jump) = (cpsr, write s dst (read s (HD src) >> w2n (read s (HD (TL src)))))) /\
+  (decode_op (pc,cpsr,s) (ROR,SOME dst,src,jump) = (cpsr, write s dst (read s (HD src) #>> w2n (read s (HD (TL src)))))) /\
+  (decode_op (pc,cpsr,s) (LDR,SOME dst,src,jump) = (cpsr, write s dst (read s (HD src)))) /\
+  (decode_op (pc,cpsr,s) (STR,SOME dst,src,jump) = (cpsr, write s (HD src) (read s dst))) /\
+  (decode_op (pc,cpsr,s) (LDMFD, SOME (REG r),src,jump) =
               (cpsr, FST (FOLDL
                           (\(s1,i) reg.
                              (write s1 reg (read s (MEM (r,POS (i + 1)))),
                               i + 1)) (s,0) src))) /\
-  (decode1 (pc,cpsr,s) (LDMFD,SOME (WREG r),src,jump) =
+  (decode_op (pc,cpsr,s) (LDMFD,SOME (WREG r),src,jump) =
               (cpsr, write (FST
                              (FOLDL
                                (\(s1,i) reg.
@@ -392,97 +337,96 @@ val decode1_thm = Q.store_thm
                                    (read s (MEM (r,POS (i + 1)))),i + 1))
                                (s,0) src)) (REG r)
                        	     (read s (REG r) + n2w (LENGTH src)))) /\
-  (decode1 (pc,cpsr,s) (STMFD,SOME (REG r),src,jump) =
+  (decode_op (pc,cpsr,s) (STMFD,SOME (REG r),src,jump) =
                   (cpsr, FST (FOLDL
                           (\(s1,i) reg.
                              (write s1 (MEM (r,NEG i)) (read s reg),i + 1))
                           (s,0) (REVERSE src)))) /\
-  (decode1 (pc,cpsr,s) (STMFD,SOME (WREG r),src,jump) =
+  (decode_op (pc,cpsr,s) (STMFD,SOME (WREG r),src,jump) =
                   (cpsr, write (FST
                           (FOLDL
                              (\(s1,i) reg.
                                 (write s1 (MEM (r,NEG i)) (read s reg),
                                  i + 1)) (s,0) (REVERSE src))) (REG r)
                        (read s (REG r) - n2w (LENGTH src)))) /\
-  (decode1 (pc,cpsr,s) (MRS,SOME dst,src,jump) = (cpsr,write s dst cpsr)) /\
-  (decode1 (pc,cpsr,s) (MSR,NONE,src,jump) = (read s (HD src),s)) /\
-  (decode1 (pc,cpsr,s) (B,NONE,src,jump) = (cpsr,write s (REG 15) (n2w (goto (pc,jump))))) /\
-  (decode1 (pc,cpsr,s) (BL,NONE,src,jump) = (cpsr,write (write s (REG 14) (n2w (pc+1))) (REG 15)
-                                                    (n2w (goto (pc,jump)))))`,
+  (decode_op (pc,cpsr,s) (MRS,SOME dst,src,jump) = (cpsr,write s dst cpsr)) /\
+  (decode_op (pc,cpsr,s) (MSR,NONE,src,jump) = (read s (HD src),s)) /\
+  (decode_op (pc,cpsr,s) (B,NONE,src,jump) = (cpsr,s)) /\
+  (decode_op (pc,cpsr,s) (BL,NONE,src,jump) = (cpsr,write s (REG 14) (n2w (SUC pc))))`,
  
-   RW_TAC std_ss [decode1_def]);
+   RW_TAC std_ss [decode_op_def]);
   
 
-  
-val decode2_def =
+val decode_cond_def = 
   Define `
-    decode2 ((pc,cpsr,s):STATE) (((op,cond,sflag), dst, src, jump):INST) =
+    decode_cond ((pc,cpsr,s):STATE) (((op,cond,sflag), dst, src, jump):INST) =
         case cond of
-            NONE -> set_pc (decode1 (pc,cpsr,s) (op,dst,src,jump)) (pc+1)
+            NONE -> (pc+1, decode_op (pc,cpsr,s) (op,dst,src,jump))
                 ||
             SOME c -> 
 		(case c of 
-		     EQ -> if getS cpsr SZ then read_pc (decode1 (pc,cpsr,s) (op,dst,src,jump))
-			    else (pc+1, cpsr, write s (REG 15) (n2w (pc+1)))
+		     EQ -> if getS cpsr SZ then (goto(pc,jump), decode_op (pc,cpsr,s) (op,dst,src,jump))
+			    else (pc+1, cpsr, s)
 		 ||  
-		     NE -> if getS cpsr SZ then (pc+1, cpsr, write s (REG 15) (n2w (pc+1)))
-                            else read_pc (decode1 (pc,cpsr,s) (op,dst,src,jump))
+		     NE -> if getS cpsr SZ then (pc+1, cpsr, s)
+                            else (goto(pc,jump), decode_op (pc,cpsr,s) (op,dst,src,jump))
                  ||
-            	     GT -> if getS cpsr SC then read_pc (decode1 (pc,cpsr,s) (op,dst,src,jump))
-			   else (pc+1, cpsr, write s (REG 15) (n2w (pc+1)))
+            	     GT -> if getS cpsr SC then (goto(pc,jump), decode_op (pc,cpsr,s) (op,dst,src,jump))
+			   else (pc+1, cpsr, s)
                  ||
-            	     LE -> if getS cpsr SC then (pc+1, cpsr, write s (REG 15) (n2w (pc+1)))
-			   else read_pc (decode1 (pc,cpsr,s) (op,dst,src,jump))
+            	     LE -> if getS cpsr SC then (pc+1, cpsr, s)
+			   else (goto(pc,jump), decode_op (pc,cpsr,s) (op,dst,src,jump))
                  ||
-            	     GE -> if getS cpsr SN then (pc+1, cpsr, write s (REG 15) (n2w (pc+1)))
-                                     else read_pc (decode1 (pc,cpsr,s) (op,dst,src,jump))
+            	     GE -> if getS cpsr SN then (pc+1, cpsr, s)
+                                     else (goto(pc,jump), decode_op (pc,cpsr,s) (op,dst,src,jump))
                  ||  
-	             LT -> if getS cpsr SN then read_pc (decode1 (pc,cpsr,s) (op,dst,src,jump))
-                                     else (pc+1, cpsr, write s (REG 15) (n2w (pc+1)))
+	             LT -> if getS cpsr SN then (goto(pc,jump), decode_op (pc,cpsr,s) (op,dst,src,jump))
+                                     else (pc+1, cpsr, s)
                  ||
-		     AL -> read_pc (decode1 (pc,cpsr,s) (op,dst,src,jump))
+		     AL -> (goto(pc,jump), decode_op (pc,cpsr,s) (op,dst,src,jump))
                  ||
-                     NV -> (pc+1, cpsr, write s (REG 15) (n2w (pc+1)))
+                     NV -> (pc+1, cpsr, s)
 		)
   `;
 
-val decode2_thm = Q.store_thm
-( "decode2_thm",
+val decode_cond_thm = Q.store_thm
+( "decode_cond_thm",
   `!pc cpsr s op sflag dst src jump.
-  (decode2 (pc,cpsr,s) ((op,NONE,sflag),dst,src,jump) = set_pc (decode1 (pc,cpsr,s) (op,dst,src,jump)) (pc + 1)) /\
-  (decode2 (pc,cpsr,s) ((op,SOME EQ,sflag),dst,src,jump) =
-              (if getS cpsr SZ then
-                 read_pc (decode1 (pc,cpsr,s) (op,dst,src,jump))
+  (decode_cond (pc,cpsr,s) ((op,NONE,sflag),dst,src,jump) = (pc+1, decode_op (pc,cpsr,s) (op,dst,src,jump))) /\
+  (decode_cond (pc,cpsr,s) ((op,SOME EQ,sflag),dst,src,jump) =
+              if getS cpsr SZ then
+                   (goto(pc,jump), decode_op (pc,cpsr,s) (op,dst,src,jump))
                else
-                 (pc + 1,cpsr,write s (REG 15) (n2w (pc + 1))))) /\
-  (decode2 (pc,cpsr,s) ((op,SOME NE,sflag),dst,src,jump) =
-              (if getS cpsr SZ then
-                 (pc + 1,cpsr,write s (REG 15) (n2w (pc + 1)))
-               else
-                 read_pc (decode1 (pc,cpsr,s) (op,dst,src,jump)))) /\
-  (decode2 (pc,cpsr,s) ((op,SOME GE,sflag),dst,src,jump) =
-              (if getS cpsr SN then
-                 (pc + 1,cpsr,write s (REG 15) (n2w (pc + 1)))
-               else
-                 read_pc (decode1 (pc,cpsr,s) (op,dst,src,jump)))) /\
-  (decode2 (pc,cpsr,s) ((op,SOME LE,sflag),dst,src,jump) =
-              (if getS cpsr SC then
-                 (pc + 1,cpsr,write s (REG 15) (n2w (pc + 1)))
-               else
-                 read_pc (decode1 (pc,cpsr,s) (op,dst,src,jump)))) /\
-  (decode2 (pc,cpsr,s) ((op,SOME GT,sflag),dst,src,jump) =
-              (if getS cpsr SC then
-                 read_pc (decode1 (pc,cpsr,s) (op,dst,src,jump))
-               else
-                 (pc + 1,cpsr,write s (REG 15) (n2w (pc + 1))))) /\
-  (decode2 (pc,cpsr,s) ((op,SOME LT,sflag),dst,src,jump) =
-              (if getS cpsr SN then
-                 read_pc (decode1 (pc,cpsr,s) (op,dst,src,jump))
-               else
-                 (pc + 1,cpsr,write s (REG 15) (n2w (pc + 1))))) /\
-  (decode2 (pc,cpsr,s) ((op,SOME AL,sflag),dst,src,jump) = read_pc (decode1 (pc,cpsr,s) (op,dst,src,jump))) /\
-  (decode2 (pc,cpsr,s) ((op,SOME NV,sflag),dst,src,jump) = (pc + 1,cpsr,write s (REG 15) (n2w (pc + 1))))`,
-  RW_TAC std_ss [decode2_def]);
+                   (pc+1, cpsr, s)) /\
+  (decode_cond (pc,cpsr,s) ((op,SOME NE,sflag),dst,src,jump) =
+              if getS cpsr SZ then
+                 (pc+1, cpsr, s)
+              else
+                 (goto(pc,jump), decode_op (pc,cpsr,s) (op,dst,src,jump))) /\
+  (decode_cond (pc,cpsr,s) ((op,SOME GE,sflag),dst,src,jump) =
+              if getS cpsr SN then
+                 (pc+1, cpsr, s)
+              else
+                 (goto(pc,jump), decode_op (pc,cpsr,s) (op,dst,src,jump))) /\
+  (decode_cond (pc,cpsr,s) ((op,SOME LE,sflag),dst,src,jump) =
+              if getS cpsr SC then
+                 (pc+1, cpsr, s)
+              else
+                 (goto(pc,jump), decode_op (pc,cpsr,s) (op,dst,src,jump))) /\
+  (decode_cond (pc,cpsr,s) ((op,SOME GT,sflag),dst,src,jump) =
+              if getS cpsr SC then
+                 (goto(pc,jump), decode_op (pc,cpsr,s) (op,dst,src,jump))
+              else
+                 (pc+1, cpsr, s)) /\
+  (decode_cond (pc,cpsr,s) ((op,SOME LT,sflag),dst,src,jump) =
+              if getS cpsr SN then
+                 (goto(pc,jump), decode_op (pc,cpsr,s) (op,dst,src,jump))
+              else
+                 (pc+1, cpsr, s)) /\
+  (decode_cond (pc,cpsr,s) ((op,SOME AL,sflag),dst,src,jump) = (goto(pc,jump), decode_op (pc,cpsr,s) (op,dst,src,jump))) /\
+  (decode_cond (pc,cpsr,s) ((op,SOME NV,sflag),dst,src,jump) = (pc+1, cpsr, s))`,
+
+  RW_TAC std_ss [decode_cond_def]);
 
 
 (*---------------------------------------------------------------------------------*)
@@ -491,45 +435,61 @@ val decode2_thm = Q.store_thm
 
 (* upload and uploadCode: upload the instructions into the instruction buffer beginning from start                                      *)
 (* By default, the code is uploaded to the buffer starting from address 0 (this is what the uploadCode describes                        *)
-                                     
-val upload_def =
-  Define `  
-    (upload (stm::rest) iB start =
-        \addr. if addr = start then stm
-               else (upload rest iB (SUC start)) addr) /\
+
+val upload_def = Define `
+    (upload (stm::stmL) iB start = upload stmL (\addr. if addr = start then stm else iB addr) (SUC start)) /\
     (upload ([]) iB start = iB)
   `;
-                
+
+
+val UPLOAD_NOT_AFFECT_LOWER = Q.store_thm (
+   "UPLOAD_NOT_AFFECT_LOWER",
+  `!instL iB start n. n < start ==>
+        ((upload instL iB start) n = iB n)`,
+   Induct_on `instL` THEN 
+   RW_TAC std_ss [upload_def] THEN
+   Induct_on `n` THEN
+   RW_TAC std_ss [upload_def] THEN           
+   `SUC n < SUC start` by RW_TAC arith_ss [] THEN
+   RES_TAC THEN
+   POP_ASSUM (K ALL_TAC) THEN
+   POP_ASSUM (ASSUME_TAC o Q.SPEC `(\addr:num. if addr = start then h else iB addr)`) THEN
+   FULL_SIMP_TAC arith_ss []
+   );
+
 val UPLOAD_LEM = Q.store_thm (
-  "UPLOAD_LEM",
-  `!instL start instB addr. addr < LENGTH instL ==>
-	((upload instL instB start) (start+addr) = (upload instL instB 0) addr)`,
-  Induct_on `addr` THEN Induct_on `instL` THEN RW_TAC list_ss [upload_def] THEN
-  Induct_on `start` THEN RW_TAC list_ss [] THEN
-  METIS_TAC [SUC_ADD_SYM, ADD_SYM]
+   "UPLOAD_LEM",
+   `!instL iB start n. n < LENGTH instL ==>
+        ((upload instL iB start) (start+n) = EL n instL)`,
+    Induct_on `n` THEN Induct_on `instL` THEN RW_TAC list_ss [upload_def] THENL [
+        RW_TAC arith_ss [UPLOAD_NOT_AFFECT_LOWER],
+        RES_TAC THEN 
+          POP_ASSUM (ASSUME_TAC o Q.SPECL [`SUC start`,`(\addr. if addr = start then h else iB addr)`]) THEN
+          METIS_TAC [ADD_SUC, SUC_ADD_SYM, ADD_SYM]
+    ]
+   );
+
+val UPLOAD_START_POINT_INDEPENDENT = Q.store_thm (
+  "UPLOAD_START_POINT_INDEPENDENT",
+  `!instL start1 start2 iB addr. addr < LENGTH instL ==>
+	((upload instL iB start1) (start1+addr) = (upload instL iB start2) (start2+addr))`,
+   RW_TAC std_ss [UPLOAD_LEM]
   );         
 
-            
 val uploadCode_def =
   Define `uploadCode instL iB = upload instL iB 0`;
 
                                      
 val UPLOADCODE_LEM = Q.store_thm (
    "UPLOADCODE_LEM",
-   `!instL instB n. n < LENGTH instL ==>
-        ((uploadCode instL instB) n = EL n instL)`,
-    SIMP_TAC list_ss [uploadCode_def] THEN Induct_on `n` THEN
-    Induct_on `instL` THEN RW_TAC list_ss [upload_def, LENGTH] THEN
-    METIS_TAC [SUC_ONE_ADD, UPLOAD_LEM, ADD_SYM]
+   `!instL iB n. n < LENGTH instL ==>
+        ((uploadCode instL iB) n = EL n instL)`,
+    RW_TAC std_ss [uploadCode_def] THEN
+    IMP_RES_TAC UPLOAD_LEM THEN
+    POP_ASSUM (ASSUME_TAC o Q.SPECL [`0`,`iB`]) THEN
+    FULL_SIMP_TAC arith_ss []
    );
         
-val UPLOAD_THM = Q.store_thm (
-    "UPLOAD_THM",
-   `!instL instB n. n < LENGTH instL ==>
-        ((upload instL instB start) (start+n) = EL n instL)`,
-    METIS_TAC [uploadCode_def, UPLOAD_LEM, UPLOADCODE_LEM ]
-   );
-
 val uploadSeg_def = Define `
     (uploadSeg 0 segs iB = iB) /\
     (uploadSeg (SUC n) segs iB = 
@@ -554,7 +514,7 @@ val (run_def,run_ind) =
         if n = 0 then (pc,cpsr,st)
         else
 	   if P (pc,cpsr,st) then (pc,cpsr,st)
-           else run (n-1) instB P (decode2 (pc,cpsr,st) (instB pc))`,
+           else run (n-1) instB P (decode_cond (pc,cpsr,st) (instB pc))`,
     WF_REL_TAC `measure FST`);
 
 val _ = save_thm("run_def", run_def);
@@ -565,7 +525,7 @@ val RUN_LEM_1 = Q.store_thm
    `!n instB s.
         (run (SUC n) instB P s =
 		if P s then s
-                else run n instB P (decode2 s (instB (FST s)))
+                else run n instB P (decode_cond s (instB (FST s)))
         ) /\
         (run 0 instB P s = s)`,
    SIMP_TAC list_ss [FORALL_STATE] THEN REPEAT GEN_TAC THEN
@@ -593,14 +553,6 @@ val RUN_THM_1 = Q.store_thm
         ASM_REWRITE_TAC [] THEN RW_TAC list_ss [RUN_LEM_1] THEN
 	RW_TAC list_ss [RUN_LEM_2]
   	]
-  );
-
-val RUN_THM_2 = Q.store_thm
-  ("RUN_THM_2",
-   `!m n s instB P. m <= n ==>
-        (run n instB P s = run (n-m) instB P (run m instB P s))`,
-  RW_TAC list_ss [FORALL_INSTM] THEN `?k. n = k + m` by PROVE_TAC [LESS_EQUAL_ADD, ADD_SYM] THEN
-  ASM_REWRITE_TAC [] THEN METIS_TAC [SUB_ADD, RUN_THM_1, ADD_SYM]
   );
 
 val _ = Globals.priming := NONE;
@@ -634,20 +586,23 @@ val LEAST_ADD_LEM = Q.store_thm
 (* Assistant theorems for the FUNPOW                                          *)
 (*----------------------------------------------------------------------------*)
 
-val FUNPOW_THM_1 = Q.prove (
+val FUNPOW_THM_1 = Q.store_thm
+  ("FUNPOW_THM_1",
   ` (!f. FUNPOW f 0 = \x.x) /\
     (!f n. FUNPOW f (SUC n) = f o (FUNPOW f n))`,
    RW_TAC list_ss [FUN_EQ_THM, FUNPOW_SUC] THEN
    RW_TAC list_ss [FUNPOW]
   );
 
-val FUNPOW_THM_2 = Q.prove (
+val FUNPOW_THM_2 = Q.store_thm
+  ("FUNPOW_THM_2",
   ` (!f. FUNPOW f 0 = \x.x) /\
     (!f n. FUNPOW f (SUC n) = (FUNPOW f n) o f)`,
    RW_TAC list_ss [FUN_EQ_THM, FUNPOW]
   );
 
-val FUNPOW_FUNPOW = Q.prove (
+val FUNPOW_FUNPOW = Q.store_thm
+  ("FUNPOW_FUNPOW",
   ` !f m n. (FUNPOW f m) o (FUNPOW f n) = FUNPOW f (m+n)`,
    Induct_on `m` THENL [
        RW_TAC list_ss [FUNPOW_THM_1] THEN
@@ -680,12 +635,21 @@ val STOPAT_THM = Q.store_thm
     Cases_on `m` THENL [
         RW_TAC std_ss [shortest_def, stopAt_def, FUNPOW],
         RW_TAC std_ss [stopAt_def,shortest_def] THEN
-        `~(n1 < LEAST n. P (FUNPOW g n x))` by METIS_TAC [Q.SPEC `\n. P(FUNPOW g n x)` LESS_LEAST] THEN
-        `SUC n <= n1` by RW_TAC arith_ss [] THEN
-        Q.EXISTS_TAC `n1 - SUC n` THEN
+        `~(n' < LEAST n. P (FUNPOW g n x))` by METIS_TAC [Q.SPEC `\n. P(FUNPOW g n x)` LESS_LEAST] THEN
+        `SUC n <= n'` by RW_TAC arith_ss [] THEN
+        Q.EXISTS_TAC `n' - SUC n` THEN
         RW_TAC arith_ss [SIMP_RULE std_ss [FUN_EQ_THM] FUNPOW_FUNPOW]
     ]
   );
+
+val SHORTEST_STOP = Q.store_thm
+  ("SHORTEST_STOP",
+   `!x P g.
+       stopAt P g x ==>
+       P (FUNPOW g (shortest P g x) x)`,
+    RW_TAC std_ss [stopAt_def, shortest_def] THEN
+    METIS_TAC [Q.SPECL [`\n. P (FUNPOW g n x)`,`x`] LEAST_INTRO]
+  );  
 
 val SHORTEST_LEM = Q.store_thm
   ("SHORTEST_LEM",
@@ -735,6 +699,25 @@ val SHORTEST_CASES = Q.store_thm
            ASSUME_TAC (DECIDE ``1 = SUC 0``) THEN
            METIS_TAC [FUNPOW, SUC_ONE_ADD, ADD_SYM]
    ]
+  );
+
+val SHORTEST_INDUCTIVE = Q.store_thm
+  ("SHORTEST_INDUCTIVE",
+   `!P g x n.
+       stopAt P g x /\
+       (shortest P g x = SUC n) ==>
+       stopAt P g (g x) /\
+       ~(P x) /\
+       (n = shortest P g (g x))`,
+    RW_TAC std_ss [] THENL [
+        `SUC 0 <= shortest P g x` by RW_TAC arith_ss [] THEN
+            METIS_TAC [Q.SPEC `SUC 0` STOPAT_THM, FUNPOW],
+        `~(shortest P g x = 0)` by RW_TAC arith_ss [] THEN
+            METIS_TAC [SHORTEST_CASES],
+        `SUC 0 <= shortest P g x` by RW_TAC arith_ss [] THEN
+             IMP_RES_TAC (Q.SPECL [`x`, `P`, `g`, `SUC 0`] SHORTEST_THM) THEN
+             FULL_SIMP_TAC arith_ss [FUNPOW]
+    ]
   );
 
 val TERD_WHILE_EQ_UNROLL = Q.store_thm
@@ -800,17 +783,80 @@ val WHILE_STILL = Q.store_thm
 (*	position. The running may not terminate and keep going on                  *) 
 (*---------------------------------------------------------------------------------*)
 
+val _ = type_abbrev("STATEPCS", Type`:STATE # (num->bool)`);
+
 val step_def = Define `
   step instB =
-       \(s,pcS).(decode2 s (instB (FST s)),FST s INSERT pcS)`;
+       \(s,pcS).(decode_cond s (instB (FST s)),FST s INSERT pcS)`;
 
 val step_FORM1 = Q.store_thm
   ("step_FORM1",
    `!instB. step instB =
-	 \s.(decode2 (FST s) (instB (FST (FST s))),FST (FST s) INSERT (SND s))`,
+	 \s.(decode_cond (FST s) (instB (FST (FST s))),FST (FST s) INSERT (SND s))`,
    RW_TAC std_ss [FUN_EQ_THM] THEN
    `?s0 pcS0. s = (s0,pcS0)` by METIS_TAC [ABS_PAIR_THM] THEN
    RW_TAC std_ss [step_def]
+  );
+
+val STATE_PCS_SEPERATE = Q.store_thm
+  ("STATE_PCS_SEPERATE",
+  `!m pcS0 pcS1 instB s. FST (FUNPOW (step instB) m (s,pcS0)) =
+                         FST (FUNPOW (step instB) m (s,pcS1))`,
+  Induct_on `m` THEN RW_TAC std_ss [FUNPOW] THEN
+  FULL_SIMP_TAC std_ss [step_def]
+  );
+
+val STOPAT_ANY_PCS = Q.store_thm
+  ("STOPAT_ANY_PCS",
+   `!pcS0 pcS1 instB j s.
+       stopAt (\s:STATEPCS. (FST s = j)) (step instB) (s,pcS0) ==>
+          stopAt (\s:STATEPCS. (FST s = j)) (step instB) (s,pcS1)`,
+    RW_TAC std_ss [stopAt_def] THEN
+    Q.EXISTS_TAC `n` THEN
+    RW_TAC std_ss [STATE_PCS_SEPERATE]
+  );
+
+val STOPAT_ANY_PCS_2 = Q.store_thm
+  ("STOPAT_ANY_PCS_2",
+   `!pcS0 pcS1 instB j s.
+       stopAt (\s:STATEPCS. (FST (FST s) = j)) (step instB) (s,pcS0) ==>
+          stopAt (\s:STATEPCS. (FST (FST s) = j)) (step instB) (s,pcS1)`,
+    RW_TAC std_ss [stopAt_def] THEN
+    Q.EXISTS_TAC `n` THEN
+    METIS_TAC [STATE_PCS_SEPERATE]
+  );
+      
+
+val SHORTEST_INDEPENDENT_OF_PCS = Q.store_thm
+  ("SHORTEST_INDEPENDENT_OF_PCS",
+  `!s0 s1 instB j.
+        stopAt (\s. FST (FST s) = j) (step instB) s0 /\ 
+        (FST s0 = FST s1) ==>
+	    (shortest (\s. FST (FST s) = j) (step instB) s0 =
+             shortest (\s. FST (FST s) = j) (step instB) s1)`,
+  Induct_on `shortest (\s. FST (FST s) = j) (step instB) s0` THENL [ 
+      RW_TAC std_ss [] THEN
+          IMP_RES_TAC SHORTEST_LEM THEN
+          FULL_SIMP_TAC std_ss [] THEN
+          `(\s. FST (FST s) = j) s1` by RW_TAC std_ss [] THEN
+          IMP_RES_TAC SHORTEST_LEM THEN
+          METIS_TAC [],
+      REWRITE_TAC [Once EQ_SYM_EQ] THEN RW_TAC std_ss [] THEN
+          IMP_RES_TAC SHORTEST_INDUCTIVE THEN
+          `?st. (?pcS0. s0 = (st,pcS0)) /\ (?pcS1. s1 = (st,pcS1))` by METIS_TAC [ABS_PAIR_THM, FST] THEN
+          Q.PAT_ASSUM `!j instB s0.p` (MP_TAC o Q.SPECL [`j`,`instB`,`step instB s0`]) THEN
+          FULL_SIMP_TAC std_ss [] THEN
+          STRIP_TAC THEN
+          POP_ASSUM (ASSUME_TAC o SIMP_RULE std_ss [Ntimes step_def 2] o (Q.SPEC `step instB (st,pcS1)`)) THEN
+	  ASM_REWRITE_TAC [] THEN
+          IMP_RES_TAC STOPAT_ANY_PCS_2 THEN
+          `~(\s. FST (FST s) = j) (st,pcS1)` by METIS_TAC [FST] THEN
+          `SUC 0 <= shortest (\s:STATEPCS. FST (FST s) = j) (step instB) (st,pcS1)` by METIS_TAC [Q.SPECL [`(st,pcS1)`,`(\s:STATEPCS. FST (FST s) = j)`,
+			`step instB`] (INST_TYPE [alpha |-> Type`:STATEPCS`] SHORTEST_LEM), DECIDE (Term `1 = SUC 0`)] THEN
+          `shortest (\s. FST (FST s) = j) (step instB) (st,pcS1)  = shortest (\s. FST (FST s) = j) (step instB) (step instB (st,pcS1)) + SUC 0`
+                by METIS_TAC [FUNPOW, SHORTEST_THM] THEN
+           RW_TAC arith_ss []
+       ]
   );
 
 val runTo_def = Define `
@@ -832,15 +878,12 @@ val runTo_FORM1 = Q.store_thm
    ]
   );
 
-   
-   
-
 val RUNTO_ADVANCE = Q.store_thm
   ("RUNTO_ADVANCE",
    `!instB j s pcS.
         (runTo instB j (s,pcS) =
                 if (FST s = j) then (s,pcS)
-                else runTo instB j (decode2 s (instB (FST s)), FST s INSERT pcS)
+                else runTo instB j (decode_cond s (instB (FST s)), FST s INSERT pcS)
         )`,
    RW_TAC list_ss [runTo_def, step_def] THENL [
         RW_TAC list_ss [Once WHILE],
@@ -848,7 +891,17 @@ val RUNTO_ADVANCE = Q.store_thm
 	]
   );
 
-val _ = type_abbrev("STATEPCS", Type`:STATE # (num->bool)`);
+val RUNTO_EXPAND_ONCE = Q.store_thm
+  ("RUNTO_EXPAND_ONCE",
+   `!instB j s.
+        (runTo instB j s =
+                if (FST (FST s) = j) then s
+                else runTo instB j (step instB s)
+        )`,
+   REPEAT STRIP_TAC THEN
+   `?s0 pcS0. s = (s0,pcS0)` by METIS_TAC [ABS_PAIR_THM] THEN
+   RW_TAC list_ss [step_def, Once RUNTO_ADVANCE]
+  );
 
 
 val UNROLL_RUNTO = Q.store_thm
@@ -864,11 +917,26 @@ val UNROLL_RUNTO = Q.store_thm
     METIS_TAC []
   );
 
+
 val terd_def = Define `
   terd instB j s =
 	stopAt (\s:STATEPCS.FST (FST s) = j) (step instB) s`;
 
+
 val set_ss = std_ss ++ SET_SPEC_ss ++ PRED_SET_ss;
+
+
+val RUNTO_STATE_PCS_SEPERATE = Q.store_thm
+  ("RUNTO_STATE_PCS_SEPERATE",
+  `!j pcS0 pcS1 instB s. 
+            stopAt (\s:STATEPCS.FST (FST s) = j) (step instB) (s,pcS0) ==>
+            (FST (runTo instB j (s,pcS0)) = FST (runTo instB j (s,pcS1)))`,
+  RW_TAC std_ss [UNROLL_RUNTO] THEN
+  IMP_RES_TAC STOPAT_ANY_PCS_2 THEN
+  RW_TAC std_ss [UNROLL_RUNTO] THEN
+  `FST (s,pcS0) = FST (s,pcS1)` by RW_TAC std_ss [] THEN
+  METIS_TAC [SHORTEST_INDEPENDENT_OF_PCS, STATE_PCS_SEPERATE]
+  );
 
 
 val RUNTO_STILL = Q.store_thm
@@ -905,7 +973,7 @@ val RUNTO_PCS_GROW = Q.store_thm
 
 val RUNTO_PCS_MEMBERS = Q.store_thm
   ("RUNTO_PCS_MEMBERS",
-   `!n m j instB s. m < n ==>
+   `!n m instB s. m < n ==>
         FST (FST (FUNPOW (step instB) m s)) IN (SND (FUNPOW(step instB) n s))`,
    Induct_on `n` THEN
    RW_TAC std_ss [] THEN
@@ -920,14 +988,72 @@ val RUNTO_PCS_MEMBERS = Q.store_thm
    ]
  );
 
-       
-val RUNTO_COMPOSITION = Q.store_thm
-  ("RUNTO_COMPOSITION",
+val RUNTO_PCS_MEMBERS_2 = Q.store_thm
+  ("RUNTO_PCS_MEMBERS_2",
+   `!n m instB s pcS. m < n ==>
+        FST (FST (FUNPOW (step instB) m (s,pcS))) IN (SND (FUNPOW(step instB) n (s,{})))`,
+   Induct_on `n` THEN
+   RW_TAC std_ss [] THEN
+   Cases_on `m = n` THENL [
+       RW_TAC std_ss [FUNPOW_SUC] THEN
+       Q.ABBREV_TAC `f = FUNPOW (step instB) m` THEN
+       RW_TAC set_ss [Once step_FORM1] THEN
+       Q.UNABBREV_TAC `f` THEN
+       METIS_TAC [STATE_PCS_SEPERATE, FST],
+       RW_TAC std_ss [FUNPOW_SUC] THEN
+       `m < n` by RW_TAC arith_ss [] THEN
+       `SND (FUNPOW (step instB) n (s,{})) SUBSET SND (FUNPOW (step instB) (SUC 0) (FUNPOW (step instB) n (s,{})))` by METIS_TAC [RUNTO_PCS_GROW]
+       THEN FULL_SIMP_TAC set_ss [FUNPOW, SUBSET_DEF]
+   ]
+ );
+
+val RUNTO_PCS_UNION_LEM = Q.store_thm
+  ("RUNTO_PCS_UNION_LEM",
+   `!n instB s pcS pcS'.
+          pcS' SUBSET SND (FUNPOW (step instB) n (s,pcS)) ==>
+          (SND (FUNPOW (step instB) n (s,pcS)) UNION pcS' =
+                  (SND (FUNPOW (step instB) n (s, pcS')) UNION pcS))`,
+   Induct_on `n` THENL [
+       RW_TAC set_ss [FUNPOW, UNION_COMM, SUBSET_UNION_ABSORPTION],
+
+       RW_TAC std_ss [FUNPOW] THEN
+       `?s1 pcS1. (step instB) (s,pcS) = (s1,pcS1)` by METIS_TAC [ABS_PAIR_THM] THEN
+       Q.PAT_ASSUM `!instB.p` (ASSUME_TAC o Q.SPECL [`instB`,`s1`,`pcS1`, `FST (s:STATE) INSERT pcS'`]) THEN
+       `FST (s:STATE) INSERT pcS' SUBSET SND (FUNPOW (step instB) n (s1,pcS1))` by (FULL_SIMP_TAC set_ss [step_def] THEN RW_TAC set_ss [INSERT_SUBSET,
+           (SIMP_RULE arith_ss [step_def] o REWRITE_RULE [FUNPOW] o Q.SPECL [`SUC n`, `0`, `instB`,`(s,pcS)`]) RUNTO_PCS_MEMBERS]) THEN
+       `step instB (s,pcS') = (s1,FST s INSERT pcS')` by FULL_SIMP_TAC std_ss [step_def] THEN
+        RES_TAC THEN
+        RW_TAC std_ss [] THEN
+       `FST (s:STATE) IN SND (FUNPOW (step instB) n (s1,FST s INSERT pcS'))` by (FULL_SIMP_TAC set_ss [step_def] THEN 
+	      RW_TAC set_ss [(SIMP_RULE arith_ss [step_def] o REWRITE_RULE [FUNPOW] o 
+              Q.SPECL [`SUC n`, `0`, `instB`,`(s,pcS')`]) RUNTO_PCS_MEMBERS, RUNTO_PCS_GROW]) THEN
+       `pcS1 = FST (s:STATE) INSERT pcS` by FULL_SIMP_TAC std_ss [step_def] THEN
+       FULL_SIMP_TAC set_ss [] THEN
+       METIS_TAC [INSERT_UNION, UNION_COMM]
+    ]
+   );
+
+
+val RUNTO_PCS_UNION = Q.store_thm
+  ("RUNTO_PCS_UNION",
+   `!n instB s pcS. 
+       stopAt (\s:STATEPCS.FST (FST s) = j) (step instB) (s,pcS) ==>
+       (SND (runTo instB j (s,pcS)) =
+            (SND (runTo instB j (s, ({}))) UNION pcS))`,
+    RW_TAC std_ss [UNROLL_RUNTO] THEN
+    IMP_RES_TAC (Q.SPECL [`pcS`,`{}`,`instB`,`j`,`s`] STOPAT_ANY_PCS_2) THEN
+    RW_TAC std_ss [UNROLL_RUNTO] THEN
+    METIS_TAC [SHORTEST_INDEPENDENT_OF_PCS, RUNTO_PCS_UNION_LEM, EMPTY_SUBSET, UNION_EMPTY, FST]
+   );
+
+
+val RUNTO_COMPOSITION_LEM = Q.store_thm
+  ("RUNTO_COMPOSITION_LEM",
    `!j k instB s0 pcS0.
         terd instB j (s0,pcS0) ==>
         let (s1,pcS1) = runTo instB j (s0,pcS0) in
-	    ~(k IN ((FST s0) INSERT pcS1)) ==>
-	        (runTo instB k (s0,pcS0) = runTo instB k (s1,pcS1))`,
+            ~(k IN ((FST s0) INSERT pcS1)) ==>
+                (runTo instB k (s0,pcS0) = runTo instB k (s1,pcS1))`,
   REPEAT GEN_TAC THEN
   Cases_on `k = j` THENL [
       RW_TAC std_ss [] THEN
@@ -945,16 +1071,16 @@ val RUNTO_COMPOSITION = Q.store_thm
           PAT_ASSUM ``!j instB pcsr regs mem pcS0. P`` (ASSUME_TAC o Q.SPECL [`j`,`instB`,`pc1`,`cpsr1`,`regs1`,`mem1`,`pcS1`]) THEN
           REPEAT STRIP_TAC THEN
           Q.ABBREV_TAC `s0 = (pc,pcsr,regs,mem)` THEN
-          Q.ABBREV_TAC `s1 = (pc1,cpsr1,regs1,mem1)` THEN  
+          Q.ABBREV_TAC `s1 = (pc1,cpsr1,regs1,mem1)` THEN
           `1 <= shortest (\s. FST (FST s) = j) (step instB) (s0,pcS0)` by RW_TAC arith_ss [] THEN
-          `shortest (\s. FST (FST s) = j) (step instB) (s0,pcS0) = 
-	      SUC (shortest (\s. FST (FST s) = j) (step instB) (s1,pcS1))` by METIS_TAC [SHORTEST_LEM, SHORTEST_CASES] THEN
+          `shortest (\s. FST (FST s) = j) (step instB) (s0,pcS0) =
+              SUC (shortest (\s. FST (FST s) = j) (step instB) (s1,pcS1))` by METIS_TAC [SHORTEST_LEM, SHORTEST_CASES] THEN
           ASM_REWRITE_TAC [FUNPOW] THEN
           FULL_SIMP_TAC std_ss [] THEN
 
-          `stopAt (\s. FST (FST s) = j) (step instB) (FUNPOW (step instB) (SUC 0) (s0,pcS0))` by 
-	       METIS_TAC [ONE, Q.SPECL [`1`,`(\s:STATEPCS. FST (FST s) = j)`] 
-			  (INST_TYPE [alpha |-> Type `:STATE # (num->bool)`] STOPAT_THM)] THEN
+          `stopAt (\s. FST (FST s) = j) (step instB) (FUNPOW (step instB) (SUC 0) (s0,pcS0))` by
+               METIS_TAC [ONE, Q.SPECL [`1`,`(\s:STATEPCS. FST (FST s) = j)`]
+                          (INST_TYPE [alpha |-> Type `:STATE # (num->bool)`] STOPAT_THM)] THEN
           POP_ASSUM MP_TAC THEN
           ASM_REWRITE_TAC [FUNPOW] THEN
           STRIP_TAC THEN RES_TAC THEN
@@ -963,14 +1089,14 @@ val RUNTO_COMPOSITION = Q.store_thm
           STRIP_TAC THEN
           Q.UNABBREV_TAC `s0` THEN
           Cases_on `pc = k` THENL [
-	      FULL_SIMP_TAC set_ss [],
+              FULL_SIMP_TAC set_ss [],
               Cases_on `v` THENL [
                   FULL_SIMP_TAC set_ss [FUNPOW] THEN
                       RW_TAC std_ss [runTo_def, Once WHILE],
-                  
+
                   ASSUME_TAC (DECIDE ``n < SUC n``) THEN
-                  `FST (FST (FUNPOW (step instB) n (s1,pcS1))) IN pcSn /\ pcS1 SUBSET SND (FUNPOW (step instB) n (s1,pcS1))` 
-		            by METIS_TAC [RUNTO_PCS_GROW, RUNTO_PCS_MEMBERS, SND] THEN
+                  `FST (FST (FUNPOW (step instB) n (s1,pcS1))) IN pcSn /\ pcS1 SUBSET SND (FUNPOW (step instB) n (s1,pcS1))`
+                            by METIS_TAC [RUNTO_PCS_GROW, RUNTO_PCS_MEMBERS, SND] THEN
                   FULL_SIMP_TAC set_ss [] THEN
                    ASSUME_TAC (DECIDE ``0 < SUC n``) THEN
                    IMP_RES_TAC RUNTO_PCS_MEMBERS THEN
@@ -978,112 +1104,28 @@ val RUNTO_COMPOSITION = Q.store_thm
                    Q.UNABBREV_TAC `s1` THEN
                    FULL_SIMP_TAC set_ss [] THEN
                    `~(k = pc1)` by (ALL_TAC THEN STRIP_TAC THEN (FULL_SIMP_TAC std_ss [IN_DEF])) THEN
-                   `runTo instB k ((pc,pcsr,regs,mem),pcS0) = runTo instB k ((pc1,cpsr1,regs1,mem1),pcS1)` by 
-				  FULL_SIMP_TAC std_ss [runTo_def, Once WHILE] THEN
+                   `runTo instB k ((pc,pcsr,regs,mem),pcS0) = runTo instB k ((pc1,cpsr1,regs1,mem1),pcS1)` by
+                                  FULL_SIMP_TAC std_ss [runTo_def, Once WHILE] THEN
                    METIS_TAC []
-	  ]
+          ]
         ]
      ]
     ]
   );
 
-
-(*----------------------------------------------------------------------------*)
-(* Run from a state until reaching another pc.                                *)
-(* The running may be trapped in a loop and not terminate                     *)
-(*----------------------------------------------------------------------------*)
-
-val runS_def = Define `
-  runS instB i j =
-     \(s,pcS). s
-	runTo instB j (s, pcS)`;
-
-
-val set_pc_LEM = Q.store_thm
-  ("set_pc_LEM",
-   `!g s:STATE. set_pc (SND s) (FST (g s)) = g s`,
-   SIMP_TAC std_ss [FORALL_STATE] THEN
-   RW_TAC list_ss [runTo_def, step_def] THENL [
-        RW_TAC list_ss [Once WHILE],
-        RW_TAC list_ss [Once WHILE]
-	]
-  );
-
-
-val RUNS_COMPOSITION = Q.store_thm
-  ("RUNS_COMPOSITION",
-   `!i j k instB s0 pcS0.
-        terS instB i j (s0,pcS0) ==>
-        let (s1,pcS1) = runS instB i j (s0,pcS0) in
-	    ~(k IN pcS1) ==> 
-	        (runS instB i k (s0,pcS0) = runS instB j k (s1,pcS1))`,
-  SIMP_TAC std_ss [runS_def, terS_def, UNROLL_RUNTO, FORALL_STATE] THEN
-  Induct_on `shortest (\(s,pcS). FST s = j) (step instB) (set_pc (pcsr,regs,mem) i,pcS0)` THENL [
-      REWRITE_TAC [Once EQ_SYM_EQ] THEN
-          RW_TAC std_ss [FUNPOW] THEN
-          FULL_SIMP_TAC std_ss [set_pc_def, write_thm] THEN
-          `(\(s,pcS).FST s = j) ((i,pcsr,regs |+ (15,n2w i),mem),pcS0)` by METIS_TAC [SHORTEST_LEM] THEN
-          FULL_SIMP_TAC std_ss [] THEN
-          SIMP_TAC finmap_ss [],
-      REWRITE_TAC [Once EQ_SYM_EQ] THEN
-          REPEAT GEN_TAC THEN
-          `?pc1 cpsr1 regs1 mem1 pcS1. step instB ((set_pc (pcsr,regs,mem) i,pcS0)) = ((pc1,cpsr1,regs1,mem1),pcS1)` by METIS_TAC [ABS_PAIR_THM] THEN
-          PAT_ASSUM ``!j instB pcsr regs mem i pcS0. P`` (ASSUME_TAC o Q.SPECL [`j`,`instB`,`cpsr1`,`regs1`,`mem1`,`i`,`pcS1`]) THEN
-          REPEAT STRIP_TAC THEN
-          `1 <= shortest (\(s,pcS). FST s = j) (step instB) (set_pc (pcsr,regs,mem) i,pcS0)` by RW_TAC arith_ss [] THEN
-          `shortest (\(s,pcS). FST s = j) (step instB) (set_pc (pcsr,regs,mem) i,pcS0) = 
-	      SUC (shortest (\(s,pcS). FST s = j) (step instB) ((pc1,cpsr1,regs1,mem1),pcS1))` by METIS_TAC [SHORTEST_LEM, SHORTEST_CASES] THEN
-          ASM_REWRITE_TAC [FUNPOW] THEN
-
-
-
-          Q.ABBREV_TAC `len = shortest (\(s,pcS). FST s = j) (step instB) (set_pc (cpsr1,regs,mem) i,pcS0)` THEN
-          
-  
-  );
-
-(*
-val RUNTO_AFTER_N_STEPS = Q.store_thm
-  ("RUNTO_AFTER_N_STEPS",
-   `!m instB byn s. runTo instB byn s = runTo instB byn (run m instB s)`,
-    Induct_on `m` THENL [
-        RW_TAC list_ss [RUN_LEM_1],
-        REPEAT STRIP_TAC THEN POP_ASSUM MP_TAC THEN 
-        ASSUME_TAC ( REWRITE_RULE [ADD_SYM, GSYM SUC_ONE_ADD] (Q.SPECL [`m`, `1`] RUN_THM_1)) THEN
-        `1 = SUC 0` by SIMP_TAC std_ss [] THEN
-        ASM_REWRITE_TAC [] THEN
-        REWRITE_TAC [Once RUN_LEM_1] THEN
-        REWRITE_TAC [Once RUN_LEM_1] THEN
-        STRIP_TAC THEN
-        Cases_on `FST (run m instB s) = byn` THENL [
-            METIS_TAC [],
-            METIS_TAC [RUNTO_LEM_1]
-        ]
-    ]
-   );
-*)
-
-(*---------------------------------------------------------------------------------*)
-(* Run to termination                                                              *)
-(*---------------------------------------------------------------------------------*)
-
-val terRun_def =
-  Define
-   `terRun (instB,byn) s = runTo instB byn s`;
-
-val TERRUN_THM = Q.store_thm
-  ("TERRUN_THM",
-   `!m s iB byn n.
-        (terRun (iB,byn) s = terRun (iB,byn) (run m (iB,byn) s))`,
-   RW_TAC arith_ss [terRun_def, RUNTO_AFTER_N_STEPS]
-  );
-
-val TERRUN_STOP = Q.store_thm
-  ("TERRUN_STOP",
-   `!s iB byn. (FST s = byn) ==>
-        (terRun (iB,byn) s = s)`,
-  RW_TAC list_ss [terRun_def] THEN
-  RW_TAC list_ss [RUNTO_LEM_2]
+       
+val RUNTO_COMPOSITION = Q.store_thm
+  ("RUNTO_COMPOSITION",
+   `!j k instB s0 pcS0 s1 pcS1.
+        terd instB j (s0,pcS0) /\ 
+        ((s1,pcS1) = runTo instB j (s0,pcS0)) /\
+	~(k IN ((FST s0) INSERT pcS1)) ==>
+	        (runTo instB k (s0,pcS0) = runTo instB k (s1,pcS1))`,
+    RW_TAC std_ss [] THEN
+    IMP_RES_TAC (SIMP_RULE std_ss [LET_THM] RUNTO_COMPOSITION_LEM) THEN
+    `?s' pcS'. runTo instB j (s0,pcS0) = (s',pcS')` by METIS_TAC [ABS_PAIR_THM] THEN
+    FULL_SIMP_TAC std_ss [] THEN
+    METIS_TAC [FST,SND]
   );
 
 (*---------------------------------------------------------------------------------*)
@@ -1113,9 +1155,23 @@ val FUPDATE_REFL = Q.store_thm
   ]
   );
 
-(*---------------------------------------------------------------------------------*)
-(* Bisimulation. Compare source codes and  ARM codes synchronously                 *)
-(*---------------------------------------------------------------------------------*)
 
+(*------------------------------------------------------------------------------------------------------*)
+(* Additional theorems for finite maps                                                                  *)
+(*------------------------------------------------------------------------------------------------------*)
+
+(* Sort in ascending order                                                                              *)
+val FUPDATE_LT_COMMUTES = Q.store_thm (
+  "FUPDATE_LT_COMMUTES",
+  ` !f a b c d. c < a ==> (f |+ (a:num, b:word32) |+ (c,d) = f |+ (c,d) |+ (a,b))`,
+    RW_TAC arith_ss [FUPDATE_COMMUTES]
+    );
+
+(* Sort in descending order                                                                             *)
+val FUPDATE_GT_COMMUTES = Q.store_thm (
+  "FUPDATE_GT_COMMUTES",
+  ` !f a b c d. c > a ==> (f |+ (a:ADDR,b:'b) |+ (c,d) = f |+ (c,d) |+ (a,b))`,
+    RW_TAC arith_ss [FUPDATE_COMMUTES]
+    );
 
 val _ = export_theory();
